% Equation 1
\begin{dmath}
{c}_{t}^{\left(-{\sigma}\right)}={\beta}\, {c}_{t+1}^{\left(-{\sigma}\right)}\, \left(1+{\alpha}\, \exp\left({a}_{t+1}\right)\, {k}_{t}^{{\alpha}-1}-{\delta}\right)
\end{dmath}
% Equation 2
\begin{dmath}
{k}_{t}={i}_{t}+\left(1-{\delta}\right)\, {k}_{t-1}
\end{dmath}
% Equation 3
\begin{dmath}
{y}_{t}=\exp\left({a}_{t}\right)\, {k}_{t-1}^{{\alpha}}
\end{dmath}
% Equation 4
\begin{dmath}
{y}_{t}={c}_{t}+{i}_{t}
\end{dmath}
% Equation 5
\begin{dmath}
{a}_{t}={\rho}\, {a}_{t-1}+{e}_{t}
\end{dmath}
